forcing.v
@@ -463,37 +463,486 @@ Defined.
 Functional Scheme force_all_ind := Induction for force_all Sort Prop.
 
 Lemma coloring_union_no_cross g p S f1 f2 :
+  undirected g ->
   (* f1 colors the induced subgraph on S *)
   coloring_ok p (subgraph_of g S) f1 ->
   (* f2 colors the complement *)
   coloring_ok p (remove_nodes g S) f2 ->
   (* No cross edges out of S *)
   S.Subset (nbs g S) S ->
+  (* f1's domain is exactly S *)
+  S.Equal (Mdomain f1) S ->
   coloring_ok p g (Munion f1 f2).
 Proof.
-  intros OK1 OK2 Closed.
+  intros Ug OK1 OK2 Closed Hdom i j Hadj.
+  (* Determine whether i is in S *)
+  destruct (SP.In_dec i S) as [HiS|HiS].
+  - (* i ∈ S: neighbor j ∈ S by closure *)
+    assert (HjS : S.In j S).
+    { apply Closed. apply nbs_spec. exists i. split; assumption. }
+    (* i has a color in f1 *)
+    assert (HiIn : M.In i f1).
+    { rewrite <- Sin_domain. rewrite Hdom. exact HiS. }
+    destruct HiIn as [ci Hci]. unfold M.MapsTo in Hci.
+    (* Use Munion_find_l to pin colors to f1 *)
+    split.
+    + intros ci' Hci'.
+      rewrite (Munion_find_l _ _ _ _ Hci) in Hci'. injection Hci' as <-.
+      assert (Hadj' : S.In j (adj (subgraph_of g S) i)).
+      { apply adj_subgraph_of_spec. auto. }
+      destruct (OK1 i j Hadj') as [Hpal _].
+      exact (Hpal ci Hci).
+    + intros ci' cj' Hci' Hcj' Heq.
+      rewrite (Munion_find_l _ _ _ _ Hci) in Hci'. injection Hci' as <-.
+      assert (HjIn : M.In j f1).
+      { rewrite <- Sin_domain. rewrite Hdom. exact HjS. }
+      destruct HjIn as [cj Hcj]. unfold M.MapsTo in Hcj.
+      rewrite (Munion_find_l _ _ _ _ Hcj) in Hcj'. injection Hcj' as <-.
+      assert (Hadj' : S.In j (adj (subgraph_of g S) i)).
+      { apply adj_subgraph_of_spec. auto. }
+      destruct (OK1 i j Hadj') as [_ Hneq].
+      exact (Hneq ci cj Hci Hcj Heq).
+  - (* i ∉ S *)
+    (* j ∉ S: if j ∈ S then i ∈ nbs g S ⊆ S, contradiction *)
+    assert (HjS : ~ S.In j S).
+    { intro HjS. apply HiS. apply Closed.
+      apply nbs_spec. exists j. split; [exact HjS|apply Ug; exact Hadj]. }
+    (* i has no color in f1, so Munion gives f2's color *)
+    assert (Hfi1 : M.find i f1 = None).
+    { destruct (M.find i f1) as [vi|] eqn:E; [|reflexivity].
+      exfalso. apply HiS. rewrite <- Hdom. apply Sin_domain.
+      exists vi. exact E. }
+    split.
+    + intros ci Hci.
+      apply Munion_case in Hci as [Hci|Hci].
+      * congruence.
+      * assert (Hadj' : S.In j (adj (remove_nodes g S) i)).
+        { apply adj_remove_nodes_spec. auto. }
+        destruct (OK2 i j Hadj') as [Hpal _].
+        exact (Hpal ci Hci).
+    + intros ci cj Hci Hcj Heq.
+      apply Munion_case in Hci as [Hci|Hci]; [congruence|].
+      assert (Hfj1 : M.find j f1 = None).
+      { destruct (M.find j f1) as [vj|] eqn:E; [|reflexivity].
+        exfalso. apply HjS. rewrite <- Hdom. apply Sin_domain.
+        exists vj. exact E. }
+      apply Munion_case in Hcj as [Hcj|Hcj]; [congruence|].
+      assert (Hadj' : S.In j (adj (remove_nodes g S) i)).
+      { apply adj_remove_nodes_spec. auto. }
+      destruct (OK2 i j Hadj') as [_ Hneq].
+      exact (Hneq ci cj Hci Hcj Heq).
+Qed.
+
+(* ---------- Helper lemmas for BFS closure ---------- *)
+
+Lemma nbs_union g A B :
+  S.Subset (nbs g (S.union A B)) (S.union (nbs g A) (nbs g B)).
+Proof.
+  intros i Hi.
+  apply nbs_spec in Hi as (v & Hv & Hiv).
+  apply S.union_spec in Hv as [Hv|Hv];
+  apply S.union_spec; [left|right]; apply nbs_spec; eauto.
+Qed.
+
+Lemma nbs_union_eq g A B :
+  S.Equal (nbs g (S.union A B)) (S.union (nbs g A) (nbs g B)).
+Proof.
+  intro i; split; intro Hi.
+  - now apply nbs_union.
+  - apply S.union_spec in Hi as [Hi|Hi];
+    apply nbs_spec in Hi as (v & Hv & Hiv);
+    apply nbs_spec; exists v; split; auto;
+    apply S.union_spec; [left|right]; auto.
+Qed.
+
+Lemma union_empty_r (s : S.t) : S.union s S.empty = s.
+Proof. destruct s; reflexivity. Qed.
+
+Lemma diff_empty_l (s : S.t) : S.diff S.empty s = S.empty.
+Proof. reflexivity. Qed.
+
+Lemma force_layers_empty_frontiers g L R k :
+  force_layers g L R S.empty S.empty k = (L, R).
+Proof.
+  induction k; simpl; auto.
+  unfold add_to_R, add_to_L.
+  rewrite nbs_empty, !diff_empty_l, !union_empty_r.
+  exact IHk.
+Qed.
+
+Lemma nbs_empty_set g s : S.Empty s -> S.Empty (nbs g s).
+Proof.
+  intros Hs x Hx. apply nbs_spec in Hx as (v & Hv & _). exact (Hs _ Hv).
+Qed.
+
+Lemma diff_empty_set s t : S.Empty s -> S.Empty (S.diff s t).
+Proof.
+  intros Hs x Hx. apply S.diff_spec in Hx as [Hx _]. exact (Hs _ Hx).
+Qed.
+
+Lemma union_empty_equal_l s t : S.Empty t -> S.Equal (S.union s t) s.
+Proof.
+  intros Ht x. rewrite S.union_spec. split.
+  - intros [H|H]; auto. exfalso; exact (Ht _ H).
+  - left; auto.
+Qed.
+
+Lemma force_layers_noop g L R FL FR k :
+  S.Empty FL -> S.Empty FR ->
+  let '(L', R') := force_layers g L R FL FR k in
+  S.Equal L' L /\ S.Equal R' R.
+Proof.
+  revert L R FL FR.
+  induction k as [|k IH]; intros L R FL FR HFL HFR; simpl.
+  - split; reflexivity.
+  - set (Vis := S.union L R).
+    assert (HnFL : S.Empty (nbs g FL)) by (apply nbs_empty_set; auto).
+    assert (HRadd : S.Empty (add_to_R g FL Vis)) by (apply diff_empty_set; auto).
+    assert (HLadd : S.Empty (add_to_L g FR Vis)).
+    { apply diff_empty_set. apply nbs_empty_set; auto. }
+    specialize (IH (S.union L (add_to_L g FR Vis))
+                   (S.union R (add_to_R g FL Vis))
+                   (add_to_L g FR Vis) (add_to_R g FL Vis) HLadd HRadd).
+    destruct (force_layers _ _ _ _ _ k) as [L' R'].
+    destruct IH as [IHL IHR].
+    split; intro x.
+    + rewrite IHL, (union_empty_equal_l L _ HLadd). reflexivity.
+    + rewrite IHR, (union_empty_equal_l R _ HRadd). reflexivity.
+Qed.
+
+(* Helper: nbs of a set split into frontier + rest *)
+Lemma nbs_split_frontier g L FL :
+  S.Subset FL L ->
+  S.Subset (nbs g L) (S.union (nbs g FL) (nbs g (S.diff L FL))).
+Proof.
+  intros HFL i Hi. apply nbs_spec in Hi as (v & Hv & Hiv).
+  destruct (SP.In_dec v FL).
+  - apply S.union_spec; left. apply nbs_spec; eauto.
+  - apply S.union_spec; right. apply nbs_spec. exists v. split; auto.
+    apply S.diff_spec; auto.
+Qed.
+
+Lemma nbs_FL_subset_vis_radd g FL Vis :
+  S.Subset (nbs g FL) (S.union Vis (add_to_R g FL Vis)).
+Proof.
+  intros x Hx.
+  destruct (SP.In_dec x Vis).
+  - apply S.union_spec; left; auto.
+  - apply S.union_spec; right. unfold add_to_R. apply S.diff_spec; auto.
+Qed.
+
+Lemma nbs_FR_subset_vis_ladd g FR Vis :
+  S.Subset (nbs g FR) (S.union Vis (add_to_L g FR Vis)).
+Proof.
+  intros x Hx.
+  destruct (SP.In_dec x Vis).
+  - apply S.union_spec; left; auto.
+  - apply S.union_spec; right. unfold add_to_L. apply S.diff_spec; auto.
+Qed.
+
+Lemma force_layers_closure g L R FL FR k :
+  undirected g ->
+  S.Subset FL L -> S.Subset FR R ->
+  S.Subset L (nodes g) -> S.Subset R (nodes g) ->
+  S.Subset (nbs g (S.diff L FL)) (S.union L R) ->
+  S.Subset (nbs g (S.diff R FR)) (S.union L R) ->
+  (S.cardinal (S.diff (nodes g) (S.union L R)) <= k)%nat ->
+  let '(L', R') := force_layers g L R FL FR k in
+  S.Subset (nbs g (S.union L' R')) (S.union L' R').
+Proof.
+  revert L R FL FR.
+  induction k as [|k IH]; intros L R FL FR Ug HFL HFR HL HR HdL HdR Hcard; simpl.
+  - (* k = 0: all nodes visited *)
+    assert (Hcover : S.Subset (nodes g) (S.union L R)).
+    { intros x Hx. destruct (SP.In_dec x (S.union L R)); auto.
+      exfalso. assert (S.In x (S.diff (nodes g) (S.union L R))) by (apply S.diff_spec; auto).
+      destruct (S.cardinal (S.diff (nodes g) (S.union L R))) eqn:Hc; [|lia].
+      apply SP.cardinal_inv_1 in Hc. apply (Hc x). auto. }
+    intros i Hi. apply nbs_spec in Hi as (v & Hv & Hiv).
+    apply Hcover. eapply nbs_subset_nodes; eauto. apply nbs_spec. eauto.
+  - (* k = S k *)
+    set (Vis := S.union L R).
+    set (Radd := add_to_R g FL Vis).
+    set (Ladd := add_to_L g FR Vis).
+    destruct (S.choose (S.union Ladd Radd)) as [fresh|] eqn:Echoose.
+    + (* Non-empty: new vertices added, use IH *)
+      assert (Hfresh : S.In fresh (S.union Ladd Radd)) by (apply S.choose_1; auto).
+      set (L' := S.union L Ladd). set (R' := S.union R Radd).
+      assert (HL' : S.Subset L' (nodes g)).
+      { unfold L'. intros x Hx. apply S.union_spec in Hx as [|Hx]; auto.
+        unfold Ladd, add_to_L in Hx. apply S.diff_spec in Hx as [Hx _].
+        eapply nbs_subset_nodes; eauto. }
+      assert (HR' : S.Subset R' (nodes g)).
+      { unfold R'. intros x Hx. apply S.union_spec in Hx as [|Hx]; auto.
+        unfold Radd, add_to_R in Hx. apply S.diff_spec in Hx as [Hx _].
+        eapply nbs_subset_nodes; eauto. }
+      assert (HdL' : S.Subset (nbs g (S.diff L' Ladd)) (S.union L' R')).
+      { assert (Hdiff_sub : S.Subset (S.diff L' Ladd) L).
+        { unfold L'. intros x Hx. apply S.diff_spec in Hx as [Hx Hx'].
+          apply S.union_spec in Hx as [|]; auto. contradiction. }
+        intros i Hi. apply (nbs_mono _ _ _ Hdiff_sub) in Hi.
+        apply (nbs_split_frontier _ _ FL HFL) in Hi.
+        apply S.union_spec in Hi as [Hi|Hi].
+        - apply (nbs_FL_subset_vis_radd g FL Vis) in Hi.
+          apply S.union_spec in Hi as [Hi|Hi].
+          * unfold Vis in Hi. apply S.union_spec in Hi as [Hi|Hi];
+            apply S.union_spec; [left; unfold L'|right; unfold R'];
+            apply S.union_spec; left; auto.
+          * apply S.union_spec; right; unfold R'; apply S.union_spec; right; auto.
+        - apply HdL in Hi. unfold Vis in Hi.
+          apply S.union_spec in Hi as [Hi|Hi];
+          apply S.union_spec; [left; unfold L'|right; unfold R'];
+          apply S.union_spec; left; auto. }
+      assert (HdR' : S.Subset (nbs g (S.diff R' Radd)) (S.union L' R')).
+      { assert (Hdiff_sub : S.Subset (S.diff R' Radd) R).
+        { unfold R'. intros x Hx. apply S.diff_spec in Hx as [Hx Hx'].
+          apply S.union_spec in Hx as [|]; auto. contradiction. }
+        intros i Hi. apply (nbs_mono _ _ _ Hdiff_sub) in Hi.
+        apply (nbs_split_frontier _ _ FR HFR) in Hi.
+        apply S.union_spec in Hi as [Hi|Hi].
+        - apply (nbs_FR_subset_vis_ladd g FR Vis) in Hi.
+          apply S.union_spec in Hi as [Hi|Hi].
+          * unfold Vis in Hi. apply S.union_spec in Hi as [Hi|Hi];
+            apply S.union_spec; [left; unfold L'|right; unfold R'];
+            apply S.union_spec; left; auto.
+          * apply S.union_spec; left; unfold L'; apply S.union_spec; right; auto.
+        - apply HdR in Hi. unfold Vis in Hi.
+          apply S.union_spec in Hi as [Hi|Hi];
+          apply S.union_spec; [left; unfold L'|right; unfold R'];
+          apply S.union_spec; left; auto. }
+      assert (Hcard' : (S.cardinal (S.diff (nodes g) (S.union L' R')) <= k)%nat).
+      { assert (Hfresh_diff : S.In fresh (S.diff (nodes g) Vis)).
+        { apply S.union_spec in Hfresh as [Hf|Hf].
+          - apply S.diff_spec; split; [apply HL'; apply S.union_spec; right; auto|].
+            unfold Ladd, add_to_L in Hf; apply S.diff_spec in Hf; tauto.
+          - apply S.diff_spec; split; [apply HR'; apply S.union_spec; right; auto|].
+            unfold Radd, add_to_R in Hf; apply S.diff_spec in Hf; tauto. }
+        assert (Hfresh_not : ~ S.In fresh (S.diff (nodes g) (S.union L' R'))).
+        { intro contra. apply S.diff_spec in contra as [_ contra].
+          apply contra. apply S.union_spec in Hfresh as [Hf|Hf];
+          apply S.union_spec; [left; unfold L'|right; unfold R'];
+          apply S.union_spec; right; auto. }
+        assert (Hsub : S.Subset (S.diff (nodes g) (S.union L' R')) (S.diff (nodes g) Vis)).
+        { unfold L', R', Vis. intros x Hx. apply S.diff_spec in Hx as [Hx1 Hx2].
+          apply S.diff_spec; split; auto. intro contra.
+          apply Hx2. apply S.union_spec in contra as [Hc|Hc];
+          apply S.union_spec; [left|right]; apply S.union_spec; left; auto. }
+        pose proof (SP.subset_cardinal_lt Hsub Hfresh_diff Hfresh_not). unfold Vis in *. lia. }
+      apply IH; auto.
+      * unfold Ladd. intros x Hx. unfold L'. apply S.union_spec; right; auto.
+      * unfold Radd. intros x Hx. unfold R'. apply S.union_spec; right; auto.
+    + (* Empty frontiers: closure holds now *)
+      assert (HLadd_empty : S.Empty Ladd).
+      { apply S.choose_2 in Echoose. intros x Hx. apply (Echoose x).
+        apply S.union_spec; left; auto. }
+      assert (HRadd_empty : S.Empty Radd).
+      { apply S.choose_2 in Echoose. intros x Hx. apply (Echoose x).
+        apply S.union_spec; right; auto. }
+      assert (HnFL : S.Subset (nbs g FL) Vis).
+      { intros x Hx. destruct (SP.In_dec x Vis); auto.
+        exfalso. apply (HRadd_empty x). unfold Radd, add_to_R.
+        apply S.diff_spec; auto. }
+      assert (HnFR : S.Subset (nbs g FR) Vis).
+      { intros x Hx. destruct (SP.In_dec x Vis); auto.
+        exfalso. apply (HLadd_empty x). unfold Ladd, add_to_L.
+        apply S.diff_spec; auto. }
+      (* nbs g (L∪R) ⊆ L∪R *)
+      assert (Hclosed : S.Subset (nbs g Vis) Vis).
+      { intros i Hi. apply nbs_union in Hi.
+        apply S.union_spec in Hi as [Hi|Hi].
+        - apply (nbs_split_frontier _ _ FL HFL) in Hi.
+          apply S.union_spec in Hi as [Hi|Hi]; auto.
+        - apply (nbs_split_frontier _ _ FR HFR) in Hi.
+          apply S.union_spec in Hi as [Hi|Hi]; auto. }
+      (* force_layers with empty frontiers doesn't change L∪R *)
+      pose proof (force_layers_noop g (S.union L Ladd) (S.union R Radd) Ladd Radd k
+                    HLadd_empty HRadd_empty) as Hnoop.
+      destruct (force_layers g (S.union L Ladd) (S.union R Radd) Ladd Radd k) as [Lf Rf].
+      destruct Hnoop as [HLf HRf].
+      (* Lf ≡ S.union L Ladd ≡ L, Rf ≡ S.union R Radd ≡ R *)
+      assert (HLf_eq : forall x, S.In x Lf <-> S.In x L).
+      { intro x. rewrite HLf. apply union_empty_equal_l; auto. }
+      assert (HRf_eq : forall x, S.In x Rf <-> S.In x R).
+      { intro x. rewrite HRf. apply union_empty_equal_l; auto. }
+      intros i Hi. apply nbs_spec in Hi as (v & Hv & Hiv).
+      apply S.union_spec in Hv as [Hv|Hv].
+      * rewrite HLf_eq in Hv. assert (S.In i Vis).
+        { apply Hclosed. apply nbs_spec. exists v. split; [apply S.union_spec; left|]; auto. }
+        unfold Vis in H. apply S.union_spec in H as [H|H];
+        apply S.union_spec; [left; apply HLf_eq|right; apply HRf_eq]; auto.
+      * rewrite HRf_eq in Hv. assert (S.In i Vis).
+        { apply Hclosed. apply nbs_spec. exists v. split; [apply S.union_spec; right|]; auto. }
+        unfold Vis in H. apply S.union_spec in H as [H|H];
+        apply S.union_spec; [left; apply HLf_eq|right; apply HRf_eq]; auto.
+Qed.
+
+Lemma reached_adj_closed g seed :
+  undirected g -> S.In seed (nodes g) ->
+  S.Subset (nbs g (reached g seed)) (reached g seed).
+Proof.
+  intros Ug Hseed.
+  unfold reached, force_component_sets.
+  pose proof (force_layers_closure g
+    (S.singleton seed) S.empty (S.singleton seed) S.empty
+    (S.cardinal (nodes g)) Ug) as H.
+  destruct (force_layers g (S.singleton seed) S.empty
+    (S.singleton seed) S.empty (S.cardinal (nodes g))) as [L' R'] eqn:E.
+  simpl in *.
+  apply H; clear H.
+  - intros x Hx; auto.
+  - intros x Hx; auto.
+  - intros x Hx. apply S.singleton_1 in Hx. subst; auto.
+  - intros x Hx. exfalso. exact (Snot_in_empty _ Hx).
+  - intros i Hi. apply nbs_spec in Hi as (v & Hv & _).
+    apply S.diff_spec in Hv as [Hv1 Hv2]. contradiction.
+  - intros i Hi. apply nbs_spec in Hi as (v & Hv & _).
+    exfalso. exact (Snot_in_empty _ Hv).
+  - apply SP.subset_cardinal. intros x Hx. apply S.diff_spec in Hx as [Hx _]. auto.
+Qed.
+
+Lemma domain_bicolor L R c1 c2 :
+  S.Equal (Mdomain (bicolor L R c1 c2)) (S.union L R).
+Proof.
+  unfold bicolor. intro i. rewrite Sin_domain. rewrite Munion_in.
   split.
-  - intros ci Hci.
-    apply Munion_case in Hci.
-    destruct Hci.
-    + unfold coloring_ok in *.
-      pose proof (OK1 i j).
-      assert (S.In j (adj (subgraph_of g S) i)).
-      {
-        admit.
-      }
-      sfirstorder.
-    + admit.
-  - intros ci cj Hfi Hfj Hadj.
-    (* Split by which branch provided the colors *)
-    apply Munion_case in Hfi; apply Munion_case in Hfj.
-    destruct Hfi as [Hi1|Hi2]; destruct Hfj as [Hj1|Hj2].
-    + (* both in S: reduce to subgraph_of g S *)
-      admit.
-    + (* i in S, j outside — impossible by closure *)
-      admit.
-    + (* symmetric to previous case *)
-      admit.
-    + (* both outside S: reduce to remove_nodes g S *)
-      admit.
-Abort.
+  - intros [Hi|Hi]; apply S.union_spec;
+    [left; rewrite <- domain_constant_color | right; rewrite <- domain_constant_color];
+    apply Sin_domain; exact Hi.
+  - intro Hi. apply S.union_spec in Hi as [Hi|Hi];
+    [left | right]; apply Sin_domain;
+    rewrite domain_constant_color; exact Hi.
+Qed.
+
+Lemma remove_nodes_undirected g s : undirected g -> undirected (remove_nodes g s).
+Proof.
+  intros Ug i j Hj.
+  apply adj_remove_nodes_spec in Hj as (Hj & Hjs & His).
+  apply adj_remove_nodes_spec. split; [|split]; auto.
+Qed.
+
+Lemma force_all_ok g c1 c2 :
+  undirected g -> bipartite g -> c1 <> c2 ->
+  coloring_ok (SP.of_list [c1;c2]) g (force_all g c1 c2).
+Proof.
+  remember (M.cardinal g) as n eqn:Hn.
+  revert g Hn.
+  induction n as [n IH] using lt_wf_ind.
+  intros g Hn Ug Hbip Hneq.
+  rewrite force_all_equation.
+  destruct (S.choose (nodes g)) as [seed|] eqn:Echoose.
+  - (* Some seed *)
+    set (LR := force_component_sets g seed).
+    set (L := fst LR). set (R := snd LR).
+    set (Sreach := S.union L R).
+    assert (Hseed : S.In seed (nodes g)) by (apply S.choose_1; auto).
+    (* reached set is closed under adjacency *)
+    assert (Hclosed : S.Subset (nbs g Sreach) Sreach).
+    { unfold Sreach, L, R, LR. apply reached_adj_closed; auto. }
+    (* force_component_ok gives coloring_ok on subgraph *)
+    pose proof (force_component_ok g seed c1 c2 Ug Hbip Hneq Hseed) as Hcomp.
+    unfold force_component, force_component_sets in Hcomp.
+    fold LR in Hcomp. fold L R in Hcomp.
+    destruct Hcomp as [Hcomp_complete Hcomp_ok].
+    (* IH for remove_nodes *)
+    assert (Hlt : (M.cardinal (remove_nodes g Sreach) < n)%nat).
+    { subst n.
+      eapply remove_nodes_lt with (i := seed).
+      - unfold Sreach, L, R, LR. apply seed_in_reached.
+      - apply FExt.in_nodes_iff. auto. }
+    assert (Hok_rem : coloring_ok (SP.of_list [c1;c2]) (remove_nodes g Sreach) (force_all (remove_nodes g Sreach) c1 c2)).
+    { apply (IH _ Hlt _ (Logic.eq_refl _)); auto.
+      - apply remove_nodes_undirected; auto.
+      - apply bipartite_remove_nodes; auto. }
+    (* domain of bicolor *)
+    assert (Hdom : S.Equal (Mdomain (bicolor L R c1 c2)) Sreach).
+    { unfold Sreach. apply domain_bicolor. }
+    (* combine using coloring_union_no_cross *)
+    apply (coloring_union_no_cross g _ Sreach); auto.
+  - (* None: empty graph *)
+    intros i j Hadj. exfalso.
+    apply S.choose_2 in Echoose.
+    assert (HiG : S.In i (nodes g)).
+    { eapply FExt.in_adj_center_in_nodes. eauto. }
+    exact (Echoose _ HiG).
+Qed.
+
+Lemma force_all_palette g c1 c2 i ci :
+  M.find i (force_all g c1 c2) = Some ci -> ci = c1 \/ ci = c2.
+Proof.
+  remember (M.cardinal g) as n eqn:Hn.
+  revert g Hn.
+  induction n as [n IH] using lt_wf_ind.
+  intros g Hn Hfi.
+  rewrite force_all_equation in Hfi.
+  destruct (S.choose (nodes g)) as [seed|] eqn:Echoose.
+  - set (LR := force_component_sets g seed) in *.
+    set (L := fst LR) in *. set (R := snd LR) in *.
+    set (Sreach := S.union L R) in *.
+    apply Munion_case in Hfi as [Hfi|Hfi].
+    + (* ci from bicolor L R c1 c2 *)
+      unfold bicolor in Hfi. apply Munion_case in Hfi as [Hfi|Hfi].
+      * left. symmetry. eapply constant_color_inv2. eauto.
+      * right. symmetry. eapply constant_color_inv2. eauto.
+    + (* ci from force_all (remove_nodes g Sreach) c1 c2 *)
+      assert (Hlt : (M.cardinal (remove_nodes g Sreach) < n)%nat).
+      { subst n. eapply remove_nodes_lt with (i := seed).
+        - unfold Sreach, L, R, LR. apply seed_in_reached.
+        - apply FExt.in_nodes_iff. apply S.choose_1 in Echoose. auto. }
+      eapply IH; eauto.
+  - rewrite WF.empty_o in Hfi. discriminate.
+Qed.
+
+Lemma reached_subset_nodes g seed :
+  undirected g -> S.In seed (nodes g) ->
+  S.Subset (reached g seed) (nodes g).
+Proof.
+  intros Ug Hseed.
+  unfold reached, force_component_sets.
+  pose proof (force_layers_subsets_nodes g
+    (S.singleton seed) S.empty (S.singleton seed) S.empty
+    (S.cardinal (nodes g)) Ug) as H.
+  destruct (force_layers g (S.singleton seed) S.empty
+    (S.singleton seed) S.empty (S.cardinal (nodes g))) as [L' R'].
+  simpl. destruct H as [HL HR].
+  - intros x Hx. apply S.singleton_1 in Hx. subst. auto.
+  - intros x Hx. exfalso. exact (Snot_in_empty _ Hx).
+  - intros x Hx. apply S.singleton_1 in Hx. subst. auto.
+  - intros x Hx. exfalso. exact (Snot_in_empty _ Hx).
+  - intros x Hx. apply S.union_spec in Hx as [Hx|Hx]; auto.
+Qed.
+
+Lemma force_all_domain g c1 c2 i ci :
+  undirected g ->
+  M.find i (force_all g c1 c2) = Some ci -> M.In i g.
+Proof.
+  remember (M.cardinal g) as n eqn:Hn.
+  revert g Hn.
+  induction n as [n IH] using lt_wf_ind.
+  intros g Hn Ug Hfi.
+  rewrite force_all_equation in Hfi.
+  destruct (S.choose (nodes g)) as [seed|] eqn:Echoose.
+  - set (LR := force_component_sets g seed) in *.
+    set (L := fst LR) in *. set (R := snd LR) in *.
+    set (Sreach := S.union L R) in *.
+    assert (Hseed : S.In seed (nodes g)) by (apply S.choose_1; auto).
+    apply Munion_case in Hfi as [Hfi|Hfi].
+    + (* i from bicolor L R c1 c2 — in reached g seed ⊆ nodes g *)
+      apply FExt.in_nodes_iff.
+      apply (reached_subset_nodes g seed Ug Hseed).
+      unfold reached, force_component_sets.
+      fold LR L R.
+      unfold bicolor in Hfi. apply Munion_case in Hfi as [Hfi|Hfi];
+      apply constant_color_inv in Hfi;
+      apply S.union_spec; [left | right]; auto.
+    + (* i from recursive call *)
+      assert (Hlt : (M.cardinal (remove_nodes g Sreach) < n)%nat).
+      { subst n. eapply remove_nodes_lt with (i := seed).
+        - unfold Sreach, L, R, LR. apply seed_in_reached.
+        - apply FExt.in_nodes_iff. auto. }
+      assert (Ug' : undirected (remove_nodes g Sreach)).
+      { apply remove_nodes_undirected. auto. }
+      assert (M.In i (remove_nodes g Sreach)).
+      { eapply IH; eauto. }
+      eapply subgraph_vert_m; [apply remove_nodes_subgraph | exact H].
+  - rewrite WF.empty_o in Hfi. discriminate.
+Qed.
